src/impl/TLS13.Impl.Client.fsti
@@ -371,6 +371,8 @@ fn process_network_bytes
                  buffer_resp.CT.consumed_len == 0sz /\
                  WS.record_prefix_incomplete (Ghost.reveal 'raw_bytes) /\
                  WS.parse_record_wire (Ghost.reveal 'raw_bytes) == None) /\
+                (buffer_resp.CT.response.CT.status == CT.StepOk ==>
+                 0 < SZ.v buffer_resp.CT.consumed_len) /\
                 (buffer_resp.CT.response.CT.status == CT.DecodeError ==>
                  buffer_resp.CT.consumed_len == 0sz) /\
                 (buffer_resp.CT.response.CT.status == CT.IllegalTransition ==>
